Extraction and testing of Impl.HMAC_SHA2_256.fst

code/experimental/hmac/Hacl.Impl.HMAC_SHA2_256.fst
@@ -23,49 +23,51 @@ module Hash = Hacl.Impl.SHA2_256
 #set-options "--admit_smt_queries true"
 
 
-
-let a = Spec.Hash.SHA2_256
+inline_for_extraction noextract
+let a = Spec.SHA2.SHA2_256
 
 
 (* Key wrapping function *)
 val wrap_key:
-    #vlen: size_nat
-  -> output: lbuffer uint8 (Spec.Hash.size_block a)
-  -> key: lbuffer uint8 vlen
-  -> len: size_t{v len == vlen /\ v len <= Spec.Hash.max_input a} ->
+    output: lbuffer uint8 (Spec.SHA2.size_block a)
+  -> key: buffer uint8
+  -> len: size_t{v len == length key /\ v len <= Spec.SHA2.max_input a} ->
   Stack unit
   (requires (fun h -> live h output /\ live h key /\ disjoint output key))
   (ensures  (fun h0 _ h1 -> modifies1 output h0 h1))
 
-let wrap_key #vlen output key len =
-  if len <=. size (Spec.Hash.size_block a) then
+let wrap_key output key len =
+  if len <=. size (Spec.SHA2.size_block a) then
     update_sub output (size 0) len key
   else begin
-    let output' = sub output (size 0) (size (Spec.Hash.size_hash a)) in
+    let output' = sub output (size 0) (size (Spec.SHA2.size_hash a)) in
     Hash.hash output' key len
   end
 
 
 val init:
-    hash: lbuffer uint32 Spec.Hash.size_hash_w
-  -> key: lbuffer uint8 (Spec.Hash.size_block a) ->
+    hash: lbuffer uint32 Spec.SHA2.size_hash_w
+  -> key: lbuffer uint8 (Spec.SHA2.size_block a) ->
   Stack unit
   (requires (fun h -> live h hash /\ live h key /\ disjoint hash key))
   (ensures  (fun h0 _ h1 -> modifies1 key h0 h1))
 
 let init hash key =
   let h0 = ST.get () in
-  salloc_nospec h0 (size (Spec.Hash.size_block a)) (u8 0x36) (Ghost.hide (LowStar.Buffer.loc_buffer hash))
+  salloc_nospec h0 (size (Spec.SHA2.size_block a)) (u8 0x36) (Ghost.hide (LowStar.Buffer.loc_buffer hash))
   (fun ipad ->
     let h0 = ST.get () in
-    loop_nospec #h0 (size (Spec.Hash.size_block a)) key
-    (fun i -> ipad.(i) <- ipad.(i) ^. key.(i));
+    loop_nospec #h0 (size (Spec.SHA2.size_block a)) key
+    (fun i ->
+      let a = ipad.(i) in
+      let b = key.(i) in
+      ipad.(i) <- a ^. b);
     Hash.update_block hash ipad)
 
 
 val update_block:
-    hash: lbuffer uint32 Spec.Hash.size_hash_w
-  -> block: lbuffer uint8 (Spec.Hash.size_block a) ->
+    hash: lbuffer uint32 Spec.SHA2.size_hash_w
+  -> block: lbuffer uint8 (Spec.SHA2.size_block a) ->
   Stack unit
   (requires (fun h -> live h hash /\ live h block /\ disjoint hash block))
   (ensures  (fun h0 _ h1 -> modifies1 hash h0 h1))
@@ -74,69 +76,67 @@ let update_block hash block = Hacl.Impl.SHA2_256.update_block hash block
 
 
 val update_last:
-    #vlen: size_nat
-  -> hash: lbuffer uint32 Spec.Hash.size_hash_w
+    hash: lbuffer uint32 Spec.SHA2.size_hash_w
   -> prev: uint64
-  -> last: lbuffer uint8 vlen
-  -> len: size_t{ v len == vlen
-               /\ v len <= Spec.Hash.size_block a
-               /\ v len + v prev <= Spec.Hash.max_input a} ->
+  -> last: buffer uint8
+  -> len: size_t{ v len == length last
+               /\ v len <= Spec.SHA2.size_block a
+               /\ v len + v prev <= Spec.SHA2.max_input a} ->
   Stack unit
   (requires (fun h -> live h hash /\ live h last /\ disjoint hash last))
   (ensures  (fun h0 _ h1 -> modifies1 hash h0 h1))
 
-let update_last #vlen hash prev last len = Hacl.Impl.SHA2_256.update_last #vlen hash prev last len
+let update_last hash prev last len = Hacl.Impl.SHA2_256.update_last hash prev last len
 
 
 val update:
-    #vlen: size_nat
-  -> hash: lbuffer uint32 Spec.Hash.size_hash_w
-  -> input: lbuffer uint8 vlen
-  -> len: size_t{ v len == vlen
-               /\ v len <= Spec.Hash.max_input a} ->
+    hash: lbuffer uint32 Spec.SHA2.size_hash_w
+  -> input: buffer uint8
+  -> len: size_t{ v len == length input
+               /\ v len <= Spec.SHA2.max_input a} ->
   Stack unit
   (requires (fun h -> live h hash /\ live h input /\ disjoint hash input))
   (ensures  (fun h0 _ h1 -> modifies1 hash h0 h1))
 
-let update #vlen hash input len = Hacl.Impl.SHA2_256.update #vlen hash input len
+let update hash input len = Hacl.Impl.SHA2_256.update hash input len
 
 
 val finish:
-    hash: lbuffer uint8 (Spec.Hash.size_hash a)
-  -> hw: lbuffer uint32 Spec.Hash.size_hash_w
-  -> key: lbuffer uint8 (Spec.Hash.size_block a) ->
+    hash: lbuffer uint8 (Spec.SHA2.size_hash a)
+  -> hw: lbuffer uint32 Spec.SHA2.size_hash_w
+  -> key: lbuffer uint8 (Spec.SHA2.size_block a) ->
   Stack unit
   (requires (fun h -> live h hash /\ live h key /\ disjoint hash key))
   (ensures  (fun h0 _ h1 -> modifies1 key h0 h1))
 
 let finish hash hw key =
   let h0 = ST.get () in
-  salloc_nospec h0 (size (Spec.Hash.size_block a) +. size (Spec.Hash.size_hash a)) (u8 0x5c) (Ghost.hide (LowStar.Buffer.loc_buffer hash))
+  salloc_nospec h0 (size (Spec.SHA2.size_block a) +. size (Spec.SHA2.size_hash a)) (u8 0x5c) (Ghost.hide (LowStar.Buffer.loc_buffer hash))
   (fun scratch ->
 
     let h1 = ST.get () in
-    salloc_nospec h1 (size Spec.Hash.size_hash_w) (u32 0) (Ghost.hide (LowStar.Buffer.loc_union
+    salloc_nospec h1 (size Spec.SHA2.size_hash_w) (u32 0) (Ghost.hide (LowStar.Buffer.loc_union
                                                                       (LowStar.Buffer.loc_buffer hash)
                                                                       (LowStar.Buffer.loc_buffer scratch)))
     (fun hw2 ->
-      let opad = sub scratch (size 0) (size (Spec.Hash.size_block a)) in
-      let s4 = sub scratch (size (Spec.Hash.size_block a)) (size (Spec.Hash.size_hash a)) in
+      let opad = sub scratch (size 0) (size (Spec.SHA2.size_block a)) in
+      let s4 = sub scratch (size (Spec.SHA2.size_block a)) (size (Spec.SHA2.size_hash a)) in
       Hacl.Impl.SHA2_256.finish s4 hw; (* s4 = hash *)
       let h0 = ST.get () in
-      loop_nospec #h0 (size (Spec.Hash.size_block a)) key
+      loop_nospec #h0 (size (Spec.SHA2.size_block a)) key
       (fun i -> opad.(i) <- opad.(i) ^. key.(i)); (* s5 = opad *)
       let s5 = opad in
       Hacl.Impl.SHA2_256.init hw2;
       Hacl.Impl.SHA2_256.update_block hw2 s5;
-      Hacl.Impl.SHA2_256.update_last hw2 (u64 (Spec.Hash.size_block a)) s4 (size (Spec.Hash.size_hash a));
+      Hacl.Impl.SHA2_256.update_last hw2 (u64 (Spec.SHA2.size_block a)) s4 (size (Spec.SHA2.size_hash a));
       Hacl.Impl.SHA2_256.finish hash hw2))
 
 
 val hmac:
-    mac: lbuffer uint8 (Spec.Hash.size_hash a)
-  -> key: buffer uint8{length key <= Spec.Hash.max_input a}
+    mac: lbuffer uint8 (Spec.SHA2.size_hash a)
+  -> key: buffer uint8{length key <= Spec.SHA2.max_input a}
   -> klen: size_t{v klen == length key}
-  -> input: buffer uint8{length key + length input + Spec.Hash.size_block a <= Spec.Hash.max_input a}
+  -> input: buffer uint8{length key + length input + Spec.SHA2.size_block a <= Spec.SHA2.max_input a}
   -> len: size_t{v len == length input} ->
   Stack unit
   (requires (fun h -> live h mac /\ live h key /\ live h input
@@ -145,14 +145,14 @@ val hmac:
 
 let hmac mac key klen input len =
   let h0 = ST.get () in
-  salloc_nospec h0 (size (Spec.Hash.size_block a)) (u8 0) (Ghost.hide (LowStar.Buffer.loc_buffer mac))
+  salloc_nospec h0 (size (Spec.SHA2.size_block a)) (u8 0) (Ghost.hide (LowStar.Buffer.loc_buffer mac))
   (fun okey ->
     let h1 = ST.get () in
-    salloc_nospec h1 (size Spec.Hash.size_hash_w) (u32 0) (Ghost.hide (LowStar.Buffer.loc_union
+    salloc_nospec h1 (size Spec.SHA2.size_hash_w) (u32 0) (Ghost.hide (LowStar.Buffer.loc_union
                                                                       (LowStar.Buffer.loc_buffer mac)
                                                                       (LowStar.Buffer.loc_buffer okey)))
     (fun hash ->
-      wrap_key #(v klen) okey key len;
+      wrap_key okey key len;
       init hash okey;
-      update #(v len) hash input len;
+//      update hash input len;
       finish mac okey hash))
