code/experimental/hmac/Hacl.HMAC_SHA2_256.fst
@@ -1,0 +1,104 @@
+module Hacl.HMAC_SHA2_256
+
+open FStar.Mul
+open FStar.HyperStack
+open FStar.HyperStack.ST
+
+open Lib.IntTypes
+open Lib.Buffer
+open Lib.ByteBuffer
+open Lib.LoopCombinators
+
+module ST = FStar.HyperStack.ST
+module Seq = Lib.Sequence
+module Loops = Lib.LoopCombinators
+
+
+module Impl = Hacl.Impl.HMAC_SHA2_256
+
+
+inline_for_extraction noextract
+let a = Spec.SHA2.SHA2_256
+
+
+(* Key wrapping function *)
+val wrap_key:
+    output: lbuffer uint8 (Spec.SHA2.size_block a)
+  -> key: buffer uint8
+  -> len: size_t{v len == length key /\ v len <= Spec.SHA2.max_input a} ->
+  Stack unit
+  (requires (fun h -> live h output /\ live h key /\ disjoint output key))
+  (ensures  (fun h0 _ h1 -> modifies1 output h0 h1))
+
+let wrap_key output key len = Impl.wrap_key output key len
+
+
+val init:
+    hash: lbuffer uint32 Spec.SHA2.size_hash_w
+  -> key: lbuffer uint8 (Spec.SHA2.size_block a) ->
+  Stack unit
+  (requires (fun h -> live h hash /\ live h key /\ disjoint hash key))
+  (ensures  (fun h0 _ h1 -> modifies1 key h0 h1))
+
+let init hash key = Impl.init hash key
+
+
+val update_block:
+    hash: lbuffer uint32 Spec.SHA2.size_hash_w
+  -> block: lbuffer uint8 (Spec.SHA2.size_block a) ->
+  Stack unit
+  (requires (fun h -> live h hash /\ live h block /\ disjoint hash block))
+  (ensures  (fun h0 _ h1 -> modifies1 hash h0 h1))
+
+let update_block hash block = Impl.update_block hash block
+
+
+val update_last:
+    hash: lbuffer uint32 Spec.SHA2.size_hash_w
+  -> prev: uint64
+  -> last: buffer uint8
+  -> len: size_t{ v len == length last
+               /\ v len <= Spec.SHA2.size_block a
+               /\ v len + v prev <= Spec.SHA2.max_input a} ->
+  Stack unit
+  (requires (fun h -> live h hash /\ live h last /\ disjoint hash last))
+  (ensures  (fun h0 _ h1 -> modifies1 hash h0 h1))
+
+let update_last hash prev last len = Impl.update_last hash prev last len
+
+
+val update:
+    hash: lbuffer uint32 Spec.SHA2.size_hash_w
+  -> input: buffer uint8
+  -> len: size_t{ v len == length input
+               /\ v len <= Spec.SHA2.max_input a} ->
+  Stack unit
+  (requires (fun h -> live h hash /\ live h input /\ disjoint hash input))
+  (ensures  (fun h0 _ h1 -> modifies1 hash h0 h1))
+
+let update hash input len = Impl.update hash input len
+
+
+val finish:
+    hash: lbuffer uint8 (Spec.SHA2.size_hash a)
+  -> hw: lbuffer uint32 Spec.SHA2.size_hash_w
+  -> key: lbuffer uint8 (Spec.SHA2.size_block a) ->
+  Stack unit
+  (requires (fun h -> live h hash /\ live h key /\ disjoint hash key))
+  (ensures  (fun h0 _ h1 -> modifies1 key h0 h1))
+
+let finish hash hw key = Impl.finish hash hw key
+
+
+val hmac:
+    mac: lbuffer uint8 (Spec.SHA2.size_hash a)
+  -> key: buffer uint8{length key <= Spec.SHA2.max_input a}
+  -> klen: size_t{v klen == length key}
+  -> input: buffer uint8{length key + length input + Spec.SHA2.size_block a <= Spec.SHA2.max_input a}
+  -> len: size_t{v len == length input} ->
+  Stack unit
+  (requires (fun h -> live h mac /\ live h key /\ live h input
+                 /\ disjoint mac key /\ disjoint mac input))
+  (ensures  (fun h0 _ h1 -> modifies1 mac h0 h1))
+
+let hmac mac key klen input len = Impl.hmac mac key klen input len
