code/experimental/hmac/Test.Impl.HMAC_SHA2_256.fst
@@ -1,0 +1,86 @@
+module Test.Impl.HMAC_SHA2_256
+
+open FStar.Mul
+open FStar.HyperStack
+open FStar.HyperStack.ST
+
+open LowStar.Buffer
+
+open Lib.IntTypes
+open Lib.Buffer
+open Lib.ByteBuffer
+open Lib.LoopCombinators
+open Lib.Print
+
+
+module Spec = Spec.SHA2
+
+module Hash = Hacl.SHA2_256
+
+inline_for_extraction let size_hash: size_nat= 32
+
+///
+/// Testing function
+///
+
+val test_hmac_sha2_256:
+    key_len: size_t
+  -> key: lbytes (size_v key_len)
+  -> msg_len: size_t
+  -> msg: lbytes (size_v msg_len)
+  -> expected: lbytes size_hash ->
+  Stack unit
+    (requires fun h -> live h msg /\ live h expected)
+    (ensures  fun h0 r h1 -> True)
+
+let test_hmac_sha2_256 key_len key msg_len msg expected =
+  push_frame();
+  let result = create #_ #size_hash (size size_hash) (u8 0xFF) in
+  Hacl.HMAC_SHA2_256.hmac result key key_len msg msg_len;
+  print_compare_display (size size_hash) result expected;
+  pop_frame()
+
+///
+/// Test 1
+///
+
+inline_for_extraction let test1_size_plaintext = 8ul
+let test1_plaintext: b:lbytes (v test1_size_plaintext){ recallable b } =
+  [@ inline_let]
+  let l:list uint8 =
+    normalize_term (List.Tot.map u8 [
+      0x48; 0x69; 0x20; 0x54; 0x68; 0x65; 0x72; 0x65
+    ])
+  in
+  assert_norm (List.Tot.length l == 8);
+  createL_global l
+
+
+let test1_expected: b:lbytes size_hash =
+  [@ inline_let]
+  let l:list uint8 =
+    normalize_term (List.Tot.map u8 [
+      0xb0; 0x34; 0x4c; 0x61; 0xd8; 0xdb; 0x38; 0x53;
+      0x5c; 0xa8; 0xaf; 0xce; 0xaf; 0x0b; 0xf1; 0x2b;
+      0x88; 0x1d; 0xc2; 0x00; 0xc9; 0x83; 0x3d; 0xa7;
+      0x26; 0xe9; 0x37; 0x6c; 0x2e; 0x32; 0xcf; 0xf7
+    ])
+  in
+  assert_norm (List.Tot.length l == 32);
+  createL_global l
+
+
+///
+/// Main
+///
+
+val main: unit -> St C.exit_code
+let main () =
+
+  C.String.print (C.String.of_literal "\nTEST 1. \n");
+  let test1_result = create #_ #size_hash (size size_hash) (u8 0x00) in
+  let test1_key = create #uint8 #20 (size 20) (u8 0x0b) in
+  Hacl.HMAC_SHA2_256.hmac test1_result test1_key (size 20) test1_plaintext test1_size_plaintext;
+  print_compare_display (size size_hash) test1_result test1_expected;
+
+  C.EXIT_SUCCESS
